theories/Graham_Scan.v
@@ -7,13 +7,13 @@ Local Open Scope Z.
 Import ListNotations.
 (* /COQ-HEAD *)
 
-(* Gift-wrapping / Jarvis' march *)
+(* Gift-wrapping / Jarvis' march / Graham Scan *)
 (* 每步查找最外侧点
    leftmost point, -y orientation =>
    append the point with minimum polar angle =>
    exit until the initial point *)
 (*
-Jarvis(x[1..n], y[1..n]):
+Graham(x[1..n], y[1..n]):
   // find leftmost point
   l = 1
   for i from 2 to n:
@@ -39,7 +39,7 @@ Jarvis(x[1..n], y[1..n]):
 (*      Main Algorithm        *)
 (* ========================== *)
 
-Fixpoint jarvis_march_inc (p : point) (T : list point) : list point :=
+Fixpoint graham_scan_inc (p : point) (T : list point) : list point :=
   match T with
   | t :: T' =>
     match T' with
@@ -49,7 +49,7 @@ Fixpoint jarvis_march_inc (p : point) (T : list point) : list point :=
       (* ccw s t p, push stack *)
       | left _ => p :: T
       (* ~ ccw s t p, pop stack & recursion *)
-      | right _ => jarvis_march_inc p T'
+      | right _ => graham_scan_inc p T'
       end
     (* T = [t], push stack *)
     | _ => p :: T
@@ -58,18 +58,19 @@ Fixpoint jarvis_march_inc (p : point) (T : list point) : list point :=
   | _ => p :: T
   end.
 
-Fixpoint jarvis_march (l: list point) : list point :=
+Fixpoint graham_scan (l: list point) : list point :=
+  (* fold_right graham_scan_inc nil l *)
   match l with
-  | p :: l' => jarvis_march_inc p (jarvis_march l')
-  | _ => l
+  | p :: l' => graham_scan_inc p (graham_scan l')
+  | _ => nil
   end.
 
 (** Simple case *)
 (*  After init,
 the vertices on T are the vertices of C_2
 in clockwise order. *)
-Theorem jarvis_convex_0 : forall (p q r : point),
-  sort_aux p [p ; q ; r] -> is_convex p (jarvis_march [p ; q ; r]).
+Theorem graham_convex_0 : forall (p q r : point),
+  sort_aux p [p ; q ; r] -> is_convex p (graham_scan [p ; q ; r]).
 Proof.
   simpl; intros.
   rewrite !Forall_ccw_cons_iff in H.
@@ -83,9 +84,9 @@ Qed.
 (*  After the i’th iteration,
 the vertices on the stack are the vertices of C_i
 in clockwise order.  *)
-(* Prove that [jarvis_march T] is subset of T retaining order *)
+(* Prove that [graham_scan T] is subset of T while preserving order *)
 Lemma succ_stack : forall (a : point) (T : list point),
-  exists T0 T', T = T0 ++ T' /\ jarvis_march_inc a T = a :: T'.
+  exists T0 T', T = T0 ++ T' /\ graham_scan_inc a T = a :: T'.
 Proof.
   intros; destruct T.
   - exists [], []. split; reflexivity.
@@ -111,13 +112,13 @@ Proof.
 Qed.
 
 Theorem Forall_ccw_conv : forall (p q : point) (T : list point),
-  Forall_ccw p q T -> Forall_ccw p q (jarvis_march T).
+  Forall_ccw p q T -> Forall_ccw p q (graham_scan T).
 Proof.
   intros.
   induction T; simpl; try eauto.
   pose proof Forall_ccw_ind p q a [] T H.
   specialize (IHT H0).
-  pose proof succ_stack a (jarvis_march T).
+  pose proof succ_stack a (graham_scan T).
   destruct H1 as [T0 [T' [H1 H2]]].
   induction T0; rewrite H1 in *; rewrite H2.
   - rewrite Forall_ccw_cons_iff in H |- *.
@@ -129,13 +130,13 @@ Proof.
 Qed.
 
 Theorem sort_aux_conv : forall (p : point) (T : list point),
-  sort_aux p T -> sort_aux p (jarvis_march T).
+  sort_aux p T -> sort_aux p (graham_scan T).
 Proof.
   intros.
   induction T; simpl; try eauto.
   pose proof sort_aux_ind p a [] T H.
   specialize (IHT H0).
-  pose proof succ_stack a (jarvis_march T).
+  pose proof succ_stack a (graham_scan T).
   destruct H1 as [T0 [T' [H1 H2]]].
   induction T0; simpl in H1; rewrite H1 in *; rewrite H2;
   destruct H; split.
@@ -152,7 +153,7 @@ Proof.
 Qed.
 
 Theorem sort_aux_convex_ind : forall (p q : point) (T : list point),
-  sort_aux p (q :: T) -> is_convex p T -> is_convex p (jarvis_march_inc q T).
+  sort_aux p (q :: T) -> is_convex p T -> is_convex p (graham_scan_inc q T).
 Proof.
   intros. destruct H.
   destruct T; try eauto.
@@ -172,14 +173,14 @@ Proof.
 Qed.
 
 
-(** Prove that if a list of point is sorted by p, then it will be convex after applying jarvis_march. *)
-Theorem jarvis_convex_1 : forall (p : point) (T : list point),
-  sort p T -> is_convex p (jarvis_march T).
+(** Prove that if a list of point is sorted by p, then it will be convex after applying graham_scan. *)
+Theorem graham_convex_1 : forall (p : point) (T : list point),
+  sort p T -> is_convex p (graham_scan T).
 Proof.
   unfold sort, sort_aux; intros. destruct H as [_ H].
   induction T; simpl; try eauto.
   pose proof sort_aux_ind p a [] T H. specialize (IHT H0).
-  pose proof sort_aux_convex_ind p a (jarvis_march T).
+  pose proof sort_aux_convex_ind p a (graham_scan T).
   apply H1; try assumption. clear H0 H1.
   simpl in *. destruct H. split.
   - apply Forall_ccw_conv. assumption.
@@ -188,7 +189,7 @@ Qed.
 
 (* ===================== *)
 
-(* TODO: check predicate *)
+(* (* TODO: check predicate *)
 (** sort -> g_ccw_list /\ consec_ccw ? *)
 Lemma sort_pred : forall p T,
   sort p T -> g_ccw_list p T /\ consec_ccw (p :: T).
@@ -201,34 +202,89 @@ Proof.
       * pose proof sort_aux_ind p a nil (p0 :: T).
         pose proof sort_ind p [a] (p0 :: T).
 (*       * rewrite consec_ccw_cons_iff in H. *)
-Abort.
+Abort. *)
 
-(*p, a: point
-  T: list point
-  H: sort_aux p (a :: T)
-  IHT: is_max_hull (jarvis_march T) T
-  ->
-  is_max_hull
-    (jarvis_march_inc a (jarvis_march T)) 
-    (a :: T) *)
+Lemma in_hull_0 : forall p T a0,
+  sort_aux p (a0 :: T) -> point_in_hull a0 p (a0 :: T).
+Proof.
+  intros.
+  destruct T; simpl; try eauto.
+  left.
+  unfold point_in_triangle. right.
+  repeat split; try apply g_ccw_rep.
+  destruct H as [? [_]]. unfold Forall_ccw in H.
+  apply Forall_cons_iff in H. destruct H as [? _].
+  apply ccw_g_ccw. apply ccw_cyclicity_2. eauto.
+Qed.
+
+(** False *)
+(* Lemma in_hull_rec : forall p T a0 q,
+  sort_aux p (a0 :: T) ->
+  point_in_hull q p (graham_scan T) ->
+  point_in_hull q p (graham_scan (a0 :: T)).
+Proof.
+  intros; simpl.
+  induction T; simpl; try eauto.
+  destruct H as [? [? ?]].
+  simpl in IHT.
+  assert (Forall_ccw a0 p T /\ sort_aux p T).
+  {
+    split; try assumption.
+    pose proof Forall_ccw_app a0 p [a] T as [? _].
+    specialize (H3 H). destruct H3 as [_ ?]; eauto.
+  }
+  specialize (IHT H3).
+  pose proof succ_stack a (graham_scan T) as [T0 [T1 [Hsp Hs]]].
+Abort. *)
+
 Lemma hull_inc : forall p a T,
   sort_aux p (a :: T) ->
-  is_max_hull (jarvis_march T) T ->
-  is_max_hull (jarvis_march_inc a (jarvis_march T)) (a :: T).
+  is_max_hull' p (graham_scan T) T ->
+  is_max_hull' p (graham_scan (a :: T)) (a :: T).
 Proof.
-  unfold sort_aux, is_max_hull; intros.
-  induction T; simpl; try eauto.
-  simpl in H0. destruct H.
-Abort.
+  unfold is_max_hull'; intros.
+  induction T. 1: { simpl. eauto. }
+  destruct H as [? [? ?]].
+  - (* ccw a0 p0 a *)
 
+(*   (*
+  IHT: Forall
+        (fun q : point =>
+         point_in_hull q p (graham_scan T)) T ->
+      Forall
+        (fun q : point =>
+         point_in_hull q p
+           (graham_scan_inc a (graham_scan T)))
+        (a :: T)
+  H3: Forall_ccw a p T
+  H4: sort_aux p (a :: T)
+  1/1
+  Forall
+    (fun q : point =>
+    point_in_hull q p
+      (graham_scan_inc a
+          (graham_scan_inc a0 (graham_scan T))))
+    (a :: a0 :: T) *)
+  (** foldr ? *)
+  assert (Forall_ccw a p T). { pose proof Forall_inv_tail H. eauto. }
+  assert (sort_aux p (a :: T)). { simpl. eauto. }
+  rewrite Forall_cons_iff in H0; destruct H0.
+  apply Forall_cons_iff; split. clear H3.
+  2: {
+    pose proof succ_stack a (graham_scan_inc a0 (graham_scan T)) as [T1 [T2 [Hsp Hi]]].
+    pose proof succ_stack a0 (graham_scan T) as [T1' [T2' [Hsp' Hi']]].
+    simpl in *.
+    apply Forall_cons_iff; split.
+    -  *)
+Admitted.
 
-Theorem jarvis_convex_2 : forall p T,
-  sort p T -> is_max_hull (jarvis_march T) T.
+Theorem graham_convex_2 : forall p T,
+  sort p T -> is_max_hull' p (graham_scan T) T.
 Proof.
   unfold sort; intros. destruct H as [_ H].
   induction T; simpl; try eauto.
-  - unfold is_max_hull; eauto.
+  - unfold is_max_hull'; eauto.
   - pose proof sort_aux_ind p a [] T H. specialize (IHT H0).
     clear H0.
-Abort.
-
+    apply hull_inc; assumption.
+Admitted.
